something new

specification/Dynamics.v
@@ -17,29 +17,37 @@ Record Lattice := {
 Section LatticeSection.
   Variable (L : Lattice).
 
+Inductive value : Type :=
+| VNat : nat -> value
+| VBool : bool -> value.
+
 Inductive tm : Type :=
 | tm_var : string -> tm
-| tm_val : nat -> tm
-| tm_bin : tm -> tm -> tm
-| tm_un : tm -> tm
+| tm_val : value -> tm
+| tm_bin_and : tm -> tm -> tm
+| tm_bin_add : tm -> tm -> tm
+| tm_bin_or : tm -> tm -> tm
+| tm_un_not : tm -> tm
 | tm_let : string -> tm -> tm -> tm
 | tm_declass : tm -> L.(carrier) -> tm.
 
-Fixpoint subst (x : string) (s : nat) (t : tm) : tm :=
+Fixpoint subst (x : string) (s : value) (t : tm) : tm :=
   match t with
   | tm_var y => if String.eqb x y then tm_val s else t
   | tm_val _ => t 
-  | tm_bin t1 t2 => tm_bin (subst x s t1) (subst x s t2)
-  | tm_un t1 => tm_un (subst x s t1)
+  | tm_bin_and t1 t2 => tm_bin_and (subst x s t1) (subst x s t2)
+  | tm_bin_add t1 t2 => tm_bin_add (subst x s t1) (subst x s t2)
+  | tm_bin_or t1 t2 => tm_bin_or (subst x s t1) (subst x s t2)
+  | tm_un_not t1 => tm_un_not (subst x s t1)
   | tm_let x_b e b =>
       let body := if String.eqb x x_b then b else (subst x s b) in
       tm_let x_b (subst x s e) body
   | tm_declass t l => tm_declass (subst x s t) l
   end.
 
-Definition smap : Type := list (string * nat).
+Definition smap : Type := list (string * value).
 
-Definition trace : Type := list (nat * L.(carrier)).
+Definition trace : Type := list (value * L.(carrier)).
 
 Fixpoint subst_many (bindings : smap) (t : tm) : tm :=
   match bindings with
@@ -61,20 +69,54 @@ Fixpoint lookup {A} (m : list (string * A)) (x : string) : option A :=
       else lookup m' x
   end.
 
-Axiom f_un : nat -> nat.
-Axiom f_bin : nat -> nat -> nat.
+Axiom f_un : value -> value.
+Axiom f_bin : value -> value -> value.
 
-Inductive big_eval : tm -> nat -> trace -> Prop := 
+Definition f_and (v1 v2 : value) : option value :=
+  match v1, v2 with
+  | VBool b1, VBool b2 => Some (VBool (andb b1 b2))
+  | _, _ => None
+  end.
+
+Definition f_add (v1 v2 : value) : option value :=
+  match v1, v2 with
+  | VNat n1, VNat n2 => Some (VNat (n1 + n2))
+  | _, _ => None 
+  end.
+
+Definition f_or (v1 v2 : value) : option value :=
+  match v1, v2 with
+  | VBool b1, VBool b2 => Some (VBool (orb b1 b2))
+  | _, _ => None
+  end.
+
+Definition f_not (v : value) : option value :=
+  match v with
+  | VBool b => Some (VBool (negb b))
+  | _ => None
+  end.
+
+Inductive big_eval : tm -> value -> trace -> Prop := 
 | Etm_val : forall v,
   big_eval (tm_val v) v []
-| Etm_un : forall e v v' tr,
-  big_eval e v tr -> v' = f_un v -> 
-  big_eval (tm_un e) v' tr
-| Etm_bin : forall e1 e2 v1 v2 v tr1 tr2,
+| Etm_un_not : forall e v v' tr,
+  big_eval e v tr -> Some v' = f_not v -> 
+  big_eval (tm_un_not e) v' tr
+| Etm_bin_and : forall e1 e2 v1 v2 v tr1 tr2,
   big_eval e1 v1 tr1 -> 
   big_eval e2 v2 tr2 -> 
-  v = f_bin v1 v2 -> 
-  big_eval (tm_bin e1 e2) v (tr1 ++ tr2)
+  Some v = f_and v1 v2 -> 
+  big_eval (tm_bin_and e1 e2) v (tr1 ++ tr2)
+| Etm_bin_add : forall e1 e2 v1 v2 v tr1 tr2,
+  big_eval e1 v1 tr1 -> 
+  big_eval e2 v2 tr2 -> 
+  Some v = f_add v1 v2 -> 
+  big_eval (tm_bin_add e1 e2) v (tr1 ++ tr2)
+| Etm_bin_or : forall e1 e2 v1 v2 v tr1 tr2,
+  big_eval e1 v1 tr1 -> 
+  big_eval e2 v2 tr2 -> 
+  Some v = f_or v1 v2 -> 
+  big_eval (tm_bin_or e1 e2) v (tr1 ++ tr2)
 | Etm_let : forall x e1 e2 v1 v2 tr1 tr2,
   big_eval e1 v1 tr1 -> 
   big_eval (subst x v1 e2) v2 tr2 -> 
@@ -83,7 +125,7 @@ Inductive big_eval : tm -> nat -> trace -> Prop :=
   big_eval e v tr ->
   big_eval (tm_declass e L) v ((v, L) :: tr). 
 
-  Theorem big_eval_det (t : tm) (v1 v2 : nat) (tr1 tr2 : trace) : 
+  Theorem big_eval_det (t : tm) (v1 v2 : value) (tr1 tr2 : trace) : 
   big_eval t v1 tr1 ->
   big_eval t v2 tr2 ->
   v1 = v2.
@@ -98,15 +140,39 @@ Inductive big_eval : tm -> nat -> trace -> Prop :=
     intros v2 tr2 h2.
     subst.
     inversion h2; subst.
-    rewrite (IHh1 _ _ H0).
+    apply IHh1 in H1 as ->.
+    rewrite <- H in H2.  
+    inversion H2; subst.
     reflexivity.
   }
   {
     intros v3 tr3 h3.
     subst.
     inversion h3; subst.
-    rewrite (IHh1_2 _ _ H2).
-    rewrite (IHh1_1 _ _ H1).
+    apply IHh1_1 in H2 as ->.
+    apply IHh1_2 in H3 as ->.
+    rewrite <- H in H6.  
+    inversion H6; subst.
+    reflexivity.
+  }
+  {
+    intros v3 tr3 h3.
+    subst.
+    inversion h3; subst.
+    apply IHh1_1 in H2 as ->.
+    apply IHh1_2 in H3 as ->.
+    rewrite <- H in H6.  
+    inversion H6; subst.
+    reflexivity.
+  }
+  {
+    intros v3 tr3 h3.
+    subst.
+    inversion h3; subst.
+    apply IHh1_1 in H2 as ->.
+    apply IHh1_2 in H3 as ->.
+    rewrite <- H in H6.  
+    inversion H6; subst.
     reflexivity.
   }
   {
@@ -135,9 +201,9 @@ Lemma subst_many_val g v :
   apply IHg.
 Qed.
 
-Lemma subst_many_tm_bin g e1 e2 : 
-  subst_many g (tm_bin e1 e2) = 
-    tm_bin (subst_many g e1) (subst_many g e2).
+Lemma subst_many_tm_bin_and g e1 e2 : 
+  subst_many g (tm_bin_and e1 e2) = 
+    tm_bin_and (subst_many g e1) (subst_many g e2).
   revert e1 e2. 
   induction g.
   simpl; reflexivity.
@@ -147,8 +213,32 @@ Lemma subst_many_tm_bin g e1 e2 :
   rewrite IHg; reflexivity.
 Qed.
 
-Lemma subst_many_un : forall g u, 
-  subst_many g (tm_un u) = tm_un (subst_many g u).
+Lemma subst_many_tm_bin_or g e1 e2 : 
+  subst_many g (tm_bin_or e1 e2) = 
+    tm_bin_or (subst_many g e1) (subst_many g e2).
+  revert e1 e2. 
+  induction g.
+  simpl; reflexivity.
+  simpl.
+  destruct a.
+  intros e1 e2.
+  rewrite IHg; reflexivity.
+Qed.
+
+Lemma subst_many_tm_bin_add g e1 e2 : 
+  subst_many g (tm_bin_add e1 e2) = 
+    tm_bin_add (subst_many g e1) (subst_many g e2).
+  revert e1 e2. 
+  induction g.
+  simpl; reflexivity.
+  simpl.
+  destruct a.
+  intros e1 e2.
+  rewrite IHg; reflexivity.
+Qed.
+
+Lemma subst_many_un_not : forall g u, 
+  subst_many g (tm_un_not u) = tm_un_not (subst_many g u).
   intros g. induction g.
   - intros u. simpl. reflexivity.
   - intros u. simpl. 
@@ -196,7 +286,7 @@ Proof.
 Qed.
 
 Lemma subst_eq_id_erasure:
-  forall (x s : string) (v n : nat) (e : tm),
+  forall (x s : string) (v n : value) (e : tm),
     x = s ->
     (subst s n (subst x v e)) = (subst x v e).
   intros.
@@ -207,6 +297,8 @@ Lemma subst_eq_id_erasure:
       reflexivity.
   - reflexivity.
   - rewrite IHe1; rewrite IHe2; reflexivity.
+  - rewrite IHe1. rewrite IHe2. reflexivity.
+  - rewrite IHe1. rewrite IHe2. reflexivity.
   - rewrite IHe; reflexivity.
   - rewrite IHe1.
     destruct (String.eqb s s0); simpl.
@@ -225,7 +317,7 @@ Lemma id_neq_sym:
 Qed.
 
 Lemma subst_neq_id_commute:
-  forall (x s : string) (v n : nat) (e : tm),
+  forall (x s : string) (v n : value) (e : tm),
     x <> s ->
     (subst s n (subst x v e)) = (subst x v (subst s n e)).
   intros.
@@ -249,6 +341,8 @@ Lemma subst_neq_id_commute:
       * rewrite H_s_s0; reflexivity.
   - reflexivity.
   - simpl; rewrite IHe1; rewrite IHe2; reflexivity.
+  - simpl; rewrite IHe1; rewrite IHe2; reflexivity.
+  - simpl; rewrite IHe1; rewrite IHe2; reflexivity.
   - simpl; rewrite IHe; reflexivity.
   - simpl; rewrite IHe1.
     destruct (String.eqb x s0); destruct (String.eqb s s0); subst; try reflexivity.
@@ -257,7 +351,7 @@ Lemma subst_neq_id_commute:
 Qed.
 
 Lemma subst_many_subst_commute:
-  forall (x : string) (v : nat) (g : smap) (e : tm),
+  forall (x : string) (v : value) (g : smap) (e : tm),
     (subst_many (filter (fun y => negb (String.eqb (fst y) x)) g) (subst x v e))
     = (subst x v (subst_many (filter (fun y => negb (String.eqb (fst y) x)) g) e)).
   induction g; simpl.
@@ -266,8 +360,8 @@ Lemma subst_many_subst_commute:
     + intro e.
       apply Bool.negb_true_iff in H_s_x. apply String.eqb_neq in H_s_x.
       apply id_neq_sym in H_s_x.
-      rewrite (subst_neq_id_commute x s v n e H_s_x).
-      rewrite (IHg (subst s n e)).
+      rewrite (subst_neq_id_commute x s v v0 e H_s_x).
+      rewrite (IHg (subst s v0 e)).
       reflexivity.
     + apply IHg.
 Qed.
