specification/Statics.v
@@ -1,6 +1,6 @@
 From Coq Require Import Strings.String.
 Require Import List.
-Import ListNotations.
+Import ListNotations .
 Require Import Dynamics.
 
 Inductive ty := 
@@ -13,29 +13,41 @@ Scheme Equality for ty.
 Section Types.
   Variable (L : Lattice).
 
-Definition context : Type := list (string *  (L.(carrier))). 
+Inductive type : Type :=
+| nat_L : L.(carrier) -> type
+| bool_L : L.(carrier) -> type.
 
-Inductive has_type : context -> tm L -> L.(carrier) -> Prop :=
+Definition context : Type := list (string *  (type)). 
+
+Inductive has_type : context -> tm L -> type -> Prop :=
 | T_Var : forall Gamma x t1,
     lookup Gamma x = Some t1 ->
     has_type Gamma (tm_var L x) t1
-| T_Val : forall Gamma v,
-    has_type Gamma (tm_val L v) L.(bot)
-| T_Un : forall Gamma e t,
-    has_type Gamma e t ->
-    has_type Gamma (tm_un L e) t
-| T_Bin : forall Gamma e1 e2 t1 t2,
-    has_type Gamma e1 t1 ->
-    has_type Gamma e2 t2 ->
-    has_type Gamma (tm_bin L e1 e2) (L.(max) t1 t2)
+| T_Val_Nat : forall Gamma v,
+    has_type Gamma (tm_val L (VNat v)) (nat_L L.(bot))
+| T_Val_Bool : forall Gamma b,
+    has_type Gamma (tm_val L (VBool b)) (bool_L L.(bot))
+| T_Un_Not : forall Gamma e l,
+    has_type Gamma e (bool_L l) ->
+    has_type Gamma (tm_un_not L e) (bool_L l)
+| T_Bin_And : forall Gamma e1 e2 l1 l2,
+    has_type Gamma e1 (bool_L l1) ->
+    has_type Gamma e2 (bool_L l2) ->
+    has_type Gamma (tm_bin_and L e1 e2) (bool_L (L.(max) l1 l2))
+| T_Bin_Add : forall Gamma e1 e2 l1 l2,
+    has_type Gamma e1 (nat_L l1) ->
+    has_type Gamma e2 (nat_L l2) ->
+    has_type Gamma (tm_bin_add L e1 e2) (nat_L (L.(max) l1 l2))
 | T_Let : forall Gamma e1 e2 x t1 t2,
     has_type Gamma e1 t1 ->
     has_type (update Gamma x t1) e2 t2 ->
     has_type Gamma (tm_let L x e1 e2) t2
-| T_Declass : forall Gamma e t Label,
-    has_type Gamma e t ->
-    has_type Gamma (tm_declass L e Label) Label.
-
+| T_Declass_Nat : forall Gamma e l Label,
+    has_type Gamma e (nat_L l) ->
+    has_type Gamma (tm_declass L e Label) (nat_L Label)
+| T_Declass_Bool : forall Gamma e l Label,
+    has_type Gamma e (bool_L l) ->
+    has_type Gamma (tm_declass L e Label) (bool_L Label).
 
 Definition base_max (t1 : ty) (t2 : ty) :=
   match t1, t2 with
